\begin{align*}
V\left(x\right)&=\frac{1}{2}kx^2\\
x_{cm}&=\frac{m_1x_1+m_2x_2}{m_1m_2}\\
\mu&=\frac{m_1m_2}{m_1+m_2}\\
\hat{H}&=\left[-\frac{\hbar^2}{2\mu} \frac{\partial^2}{\partial x^2}+ \frac{1}{2}kx^2\right]\\\
\psi_v\left(x\right)&=A_vH_v\left(\alpha^{1/2}x\right)e^{-\frac{1}{2}\alpha x^2}\\
\psi_0\left(x\right)&=\left(\frac{\alpha}{\pi}\right)^{1/4}e^{-\frac{1}{2}\alpha x^2}\\
\psi_1\left(x\right)&=\left(\frac{4\alpha^3}{\pi}\right)^{1/4}xe^{-\frac{1}{2}\alpha x^2}\\
\psi_2\left(x\right)&=\left(\frac{\alpha}{4\pi}\right)^{1/4}\left(2\alpha x^2-1\right)e^{-\frac{1}{2}\alpha x^2}\\
\alpha&=\sqrt{\frac{k\mu}{\hbar^2}}\\
%\psi_3\left(x\right)&=\left(\frac{\alpha^3}{9\pi}\right)^{1/4}\left(2\alpha x^3-3x\right)e^{-\frac{1}{2}\alpha x^2}\\
E_v&=\hbar\sqrt{\frac{k}{\mu}}\left(v+\frac{1}{2}\right)=h\nu\left(v+\frac{1}{2}\right); v = 0, 1, 2, 3, \cdots\\
\nu&=\frac{1}{2\pi}\sqrt{\frac{k}{\mu}}=\tilde{\nu}c\\
\end{align*}
%A_v&=\frac{1}{\sqrt{2^vv!}}\left(\frac{\alpha}{\pi}\right)^{1/2}\\
%H_0\left(\xi\right)&=1\\
%H_1\left(\xi\right)&=2\xi\\
%H_2\left(\xi\right)&=4\xi^2-2\\

%H_3\left(\xi\right)&=8x^3-12x\\
