\begin{align*}
%\int_{-\infty}^{+\infty} f\left(x\right) dx &= 0 \textrm{ for odd } f\left(x\right)\\
%f\left(-x\right) &= -f\left(x\right)\textrm{ for odd } f\left(x\right)\\
%\int_{-\infty}^{+\infty} f\left(x\right) dx &= 2 \int_{0}^{+\infty} f\left(x\right) dx \textrm{ for even } f\left(x\right)\\
%f\left(-x\right) &= f\left(x\right)\textrm{ for even } f\left(x\right)\\
\int \sin \left(\xi x\right) dx &= -\frac{1}{\xi} \cos \left(\xi x\right)\\
\int \cos \left(\xi x\right) dx &= \frac{1}{\xi} \sin \left(\xi x\right)\\
\int \sin^2 \left(\xi x\right) dx &= \frac{x}{2} - \frac{\sin \left(2\xi x\right)} {4\xi} \\
\int \cos^2 \left(\xi x\right) dx &= \frac{x}{2} + \frac{\sin \left(2\xi x\right)} {4\xi} \\
\int x \sin^2 \left(\xi x \right) dx &= \frac{x^2}{4} - \frac{\cos \left(2\xi x\right)}{8\xi^2} - \frac{x \sin \left(2\xi x\right)}{4\xi}\\
\int x \cos^2 \left(\xi x \right) dx &= \frac{x^2}{4} + \frac{\cos \left(2\xi x\right)}{8\xi^2} + \frac{x \sin \left(2\xi x\right)}{4\xi}\\
\int x^2 \sin^2 \left(\xi x \right) dx &= \frac{x^3}{6} - \left(\frac{x^2}{4\xi}-\frac{1}{8\xi^3}\right)\sin\left(2\xi x \right) -\frac{x}{4\xi^2}\cos\left(2\xi x\right)\\
\int x^2 \cos^2 \left(\xi x \right) dx &= \frac{x^3}{6} + \left(\frac{x^2}{4\xi}-\frac{1}{8\xi^3}\right)\sin\left(2\xi x \right) +\frac{x}{4\xi^2}\cos\left(2\xi x\right)\\
\int_0^{\infty} e^{-\xi x^2}dx &= \left(\frac{\pi}{4\xi} \right)^{1/2}\\
\int_0^\infty x^{2n}e^{-\xi x^2}dx&=\frac{1\cdot 3 \cdot 5 \cdots \left(2n-1\right)}{2^{n+1}\xi^n}\sqrt{\frac{\pi}{\xi}}\\
\int_0^\infty x^{2n+1}e^{-\xi x^2}dx&=\frac{n!}{2\xi^{n+1}}\\
\int_0^\infty x^{n}e^{-\xi x}dx&=\frac{n!}{\xi^{n+1}}\\
\end{align*}
%\int \sin^3\left(ax\right) dx &= \frac{1}{a}\left[-\cos\left(ax\right) + \frac{\cos^3\left(ax\right)}{3} \right]\\
%\int \sin^4\left(ax\right) dx &= \frac{1}{a}\left[-\frac{1}{4}\sin^3\left(ax\right)\cos\left(ax\right) + \frac{3}{8}\left(ax-\frac{1}{2}\sin\left(2ax\right) \right)\right]\\
%\int \sin^5\left(ax\right) dx &= \frac{1}{a}\left[-\cos\left(ax\right) + \frac{2\cos^3\left(ax\right)}{3} - \frac{\cos^5\left(ax\right)}{5} \right]\\
