\subsubsection{Polar}
\begin{align*}
x&=r\cos\phi\\
y&=r\sin\phi\\
r&=\sqrt{x^2+y^2}\\
\phi&=\tan^{-1}{\frac{y}{x}}\\
&\left(\frac{\partial ^2}{\partial x^2} + \frac{\partial ^2}{\partial y^2}\right)_{r=r_0} = \frac{1}{r_0^2}\frac{\partial^2}{\partial \phi^2}
\end{align*}

\subsubsection{Spherical}
\begin{align*}
x&=r\sin\theta\cos\phi\\
y&=r\sin\theta\sin\phi\\
z&=r\cos\theta\\
r&=\sqrt{x^2+y^2+z^2}\\
\theta&=\cos^{-1}\frac{z}{\sqrt{x^2+y^2+z^2}}\\
\phi&=\tan^{-1}{\frac{y}{x}}\\
dV&=dx\,dy\,dz=r^2\,\sin\theta\, dr\, d\theta\, d\phi\\
&\nabla^2_{r=r_0} = \cdots\\
&\left(\frac{\partial ^2}{\partial x^2} + \frac{\partial ^2}{\partial y^2} + \frac{\partial ^2}{\partial z^2}\right)_{r=r_0} =\cdots\\
& \frac{1}{r_0^2}\left[\frac{1}{\sin\theta}\frac{\partial}{\partial \theta}\left(\sin \theta \frac{\partial}{\partial \theta} \right)_{r,\phi} + \frac{1}{\sin^2\theta}\left(\frac{\partial^2}{\partial \phi^2} \right)_{r,\theta}\right]\\
\\
&\nabla^2=\cdots\\
&\frac{1}{r^2}\frac{\partial}{\partial r} \left( r^2 \frac{\partial}{\partial r} \right)_{\theta,\phi} + \frac{1}{r^2 \sin \theta}\frac{\partial}{\partial \theta}\left(\sin \theta \frac{\partial}{\partial \theta} \right)_{r,\phi} \cdots \\
&+ \frac{1}{r^2 \sin^2 \theta}\left(\frac{\partial^2}{\partial \phi ^2}\right)_{r,\theta}
\end{align*}
