\begin{align*}
&E=h\nu = \frac{hc}{\lambda}\\
&\lambda = \frac{h}{p}\\
&\Psi\left(x,t\right) = \psi\left(x\right)e^{-i\left(E/\hbar\right)t}\\
&\left[-\frac{\hbar^2}{2m} \nabla^2+ V\left(x,t\right)\right]\Psi\left(x,t\right) = i\hbar \frac{\partial \Psi\left(x,t\right)}{\partial t}\\
&\left[-\frac{\hbar^2}{2m} \nabla^2+ V\left(x\right)\right]\psi\left(x\right) = E\psi\left(x\right)\\
&\hat{H}\psi_n\left(x\right) = E_n\psi_n\left(x\right)\\
%&\hat{H}\Psi\left(x,t\right) = i\hbar\frac{\partial \Psi\left(x,t\right)}{\partial t}\\
&\nabla^2 = \left(\frac{\partial^2}{\partial x^2} +\frac{\partial^2}{\partial y^2} +\frac{\partial^2}{\partial z^2} \right)\\
&\hat{x}=x\\
&\hat{p_x}=-i\hbar \frac{\partial}{\partial x}\\
&\int_{-\infty}^{+\infty}\Psi^*\left(x,t\right)\Psi\left(x,t\right)dx=1\\
&\left<a\right> = \frac{\int_{-\infty}^{+\infty}\Psi^*\left(x,t\right)\hat{A}\Psi\left(x,t\right)dx}{\int_{-\infty}^{+\infty}\Psi^*\left(x,t\right)\Psi\left(x,t\right)dx}\\
&\left[\hat{A},\hat{B}\right] = \hat{A}\hat{B} - \hat{B}\hat{A}\\
&\left[\hat{A},\hat{B}\right] = -\left[\hat{B},\hat{A}\right]\\
&\Delta p\Delta x \geq \frac{\hbar}{2}\\
&E_{variational} = \frac{\int \Phi^*\hat{H}\Phi d\tau}{\int \Phi^*\Phi d\tau}\geq E_0\\
\end{align*}
