\begin{align*}
I&=\mu r^2\\
L&=I\omega\\
KE&=\frac{1}{2}I\omega^2\\
&=\frac{L^2}{2I}\\
\end{align*}

\subsubsection{2D}
\begin{align*}
\hat{H}&=-\frac{\hbar^2}{2\mu r_0^2}\frac{\partial^2}{\partial \phi^2}\\
\Phi_{m_l}\left(\phi\right)&=\frac{1}{\sqrt{2\pi}}e^{im_l\phi}\\
m_l&=0, \pm1, \pm2, \cdots\\
E_{m_l}&=\frac{\hbar^2 m_l^2}{2I}\\
\hat{L_z}\Phi_{m_l}\left(\phi\right)&=m_l\hbar \Phi_{m_l}\left(\phi\right)
\end{align*}

\subsubsection{3D}
\begin{align*}
\hat{H}=-\frac{\hbar^2}{2\mu r_0^2}&\left[\frac{1}{\sin\theta}\frac{\partial}{\partial \theta}\left(\sin \theta \frac{\partial}{\partial \theta} \right)_{r,\phi} + \frac{1}{\sin^2\theta}\left(\frac{\partial^2}{\partial \phi^2} \right)_{r,\theta}\right]\\
Y\left(\theta,\phi\right)&=Y_l^{m_l}\left(\theta,\phi\right) = \Theta_l^{m_l}\left(\theta\right)\Phi_{m_l}\left(\phi\right)\\
E_l&=\frac{\hbar^2}{2I}l\left(l+1\right)\\
l&=0, 1, 2, 3, \ldots\\
m_l&=-l, -\left(l-1\right),\ldots,0,\ldots,\left(l-1\right),l\\
E_J&=hc\tilde{B}J\left(J+1\right)\\
\tilde{B}&=\frac{h}{8\pi^2c\mu r_0^2}\\
\hat{L_z}Y_l^{m_l}\left(\theta,\phi\right) &=m_l\hbar Y_l^{m_l}\left(\theta,\phi\right)\\
\hat{L^2}Y_l^{m_l}\left(\theta,\phi\right) &=\hbar^2l\left(l+1\right) Y_l^{m_l}\left(\theta,\phi\right)\\
\hat{L}_{\begin{smallmatrix}
	x\\
	y\\
	z\\
	\end{smallmatrix}}&=-i\hbar\left(\begin{smallmatrix}
	y\\
	z\\
	x\\
	\end{smallmatrix}\frac{\partial}{\partial \begin{smallmatrix}
	z\\
	x\\
	y\\
	\end{smallmatrix}}-\begin{smallmatrix}
	z\\
	x\\
	y\\
	\end{smallmatrix}\frac{\partial}{\partial \begin{smallmatrix}
	y\\
	z\\
	x\\
	\end{smallmatrix}}\right)\\
%\hat{L_y}&=-i\hbar\left(z\frac{\partial}{\partial x}-x\frac{\partial}{\partial z}\right)\\
%\hat{L_z}&=-i\hbar\left(x\frac{\partial}{\partial y}-y\frac{\partial}{\partial x}\right)\\
\left[\hat{L}_{\begin{smallmatrix}
	x\\
	y\\
	z\\
	\end{smallmatrix}},\hat{L}_{\begin{smallmatrix}
	y\\
	z\\
	x\\
	\end{smallmatrix}}\right]&=i\hbar\hat{L}_{\begin{smallmatrix}
	z\\
	x\\
	y\\
	\end{smallmatrix}}\\
\end{align*}
%\left[\hat{L_y},\hat{L_z}\right]&=i\hbar\hat{L_x}\\
%\left[\hat{L_z},\hat{L_x}\right]&=i\hbar\hat{L_y}\\
