\subsubsection{Complex}
\begin{align*}
Y_l^{m_l}\left(\theta,\phi\right)&=\cdots\\
Y_0^0\left(\theta,\phi\right)&=\left(\frac{1}{4\pi}\right)^{1/2}\\
Y_1^0\left(\theta,\phi\right)&=\left(\frac{3}{4\pi}\right)^{1/2}\cos\theta\\
Y_1^{\pm 1}\left(\theta,\phi\right)&=\mp\left(\frac{3}{8\pi}\right)^{1/2}\sin\theta e^{\pm i \phi}\\
Y_2^0\left(\theta,\phi\right)&=\left(\frac{5}{16\pi}\right)^{1/2}\left(3\cos ^2 \theta -1 \right)\\
Y_2^{\pm 1}\left(\theta,\phi\right)&=\mp\left(\frac{15}{8\pi}\right)^{1/2}\sin\theta \cos\theta e^{\pm i \phi}\\
Y_2^{\pm 2}\left(\theta,\phi\right)&=\left(\frac{15}{32\pi}\right)^{1/2}\sin^2\theta e^{\pm 2i \phi}\\
\end{align*}
\subsubsection{Real}
\begin{align*}
p_z &= Y_1^0=\sqrt{\frac{3}{4\pi}}\cos\theta\\
p_x&=\frac{-1}{\sqrt{2}}\left( Y_1^1-Y_1^{-1}\right)= \sqrt{\frac{3}{4\pi}}\sin \theta\cos\phi\\
p_y&=\frac{-1}{\sqrt{2}i}\left( Y_1^1+Y_1^{-1}\right)= \sqrt{\frac{3}{4\pi}}\sin \theta\sin\phi\\
d_{z^2}&=Y_2^0=\sqrt{\frac{5}{16\pi}}\left(3\cos ^2 \theta -1 \right)\\
d_{xz}&=\frac{-1}{\sqrt{2}}\left( Y_2^1-Y_2^{-1}\right)=\sqrt{\frac{15}{4\pi}}\sin \theta\cos\theta\cos\phi\\
d_{yz}&=\frac{-1}{\sqrt{2}i}\left( Y_2^1+Y_2^{-1}\right)=\sqrt{\frac{15}{4\pi}}\sin \theta\cos\theta\sin\phi\\
d_{xy}&=\frac{1}{\sqrt{2}i}\left( Y_2^2-Y_2^{-2}\right)=\sqrt{\frac{15}{16\pi}}\sin^2\theta\sin 2\phi\\
d_{x^2-y^2}&=\frac{1}{\sqrt{2}}\left( Y_2^2+Y_2^{-2}\right)=\sqrt{\frac{15}{16\pi}}\sin^2\theta\cos 2\phi\\
\end{align*}
